wip recognising encoded tapes

theories/L/Complexity/Reductions/TMGenNP/mTM_to_singleTapeTM.v
@@ -1,4 +1,4 @@
-(* -*- coq-prefer-top-of-conclusion: t; -*- *)
+(** In emacs: coq-prefer-top-of-conclusion: t; *)
 From Undecidability.L Require Import Tactics.LTactics.
 From Undecidability.L.Datatypes Require Import Lists LVector.
 From Undecidability.L.Complexity Require Import NP Synthetic Monotonic.
@@ -10,6 +10,7 @@ From Undecidability.L.Complexity  Require Import LMGenNP TMGenNP_fixed_mTM.
 
 From Undecidability.TM Require Single.EncodeTapes Single.StepTM CaseList.
 
+Require Import FunInd.
 
 
 
@@ -41,7 +42,7 @@ From Coq.ssr Require Import ssrfun.
 Module CheckEncodesTape.
   Section checkEncodesTape.
 
-    Import EncodeTapes StateWhile CaseList Mono Multi MoveToSymbol Copy Switch If Combinators Option.
+    Import EncodeTapes StateWhile CaseList Mono Multi MoveToSymbol Copy Switch If Combinators.
     Context (sig:finType) (n:nat).
 
     Compute encode_tape (midtape [3;2;1] 4 [5;6;7]).
@@ -59,24 +60,44 @@ Module CheckEncodesTape.
     Definition Rel : pRel sig__M bool 1 := ContainsEncoding.Rel d__sig (encode_tape (sig:=sig)).
 
     (*MOVE*)
-    Definition isLeftBorder {sig : Type} (s : sigTape sig) : bool :=
+    Definition isNilBlank {sig : Type} (s : sigTape sig) : bool :=
       match s with
-      | LeftBlank _ | NilBlank => true
+        NilBlank => true
+      | _ => false
+      end.
+    
+    (*MOVE*)
+    Definition isLeftBlank {sig : Type} (s : sigTape sig) : bool :=
+      match s with
+      | LeftBlank _  => true
       | _ => false
       end.
 
     (*MOVE*)
-    Definition isRightBorder {sig : Type} (s : sigTape sig) : bool :=
+    Definition isRightBlank {sig : Type} (s : sigTape sig) : bool :=
       match s with
-      | RightBlank _ | NilBlank => true
+      | RightBlank _ => true
       | _ => false
       end.
 
-    Let M2 x :pTM sig__M bool 1 := if negb (Option.apply (@isMarked sig) false x)
+    (*MOVE*)
+    Definition isSymbol {sig : Type} (s : sigTape sig) : bool :=
+      match s with
+      | UnmarkedSymbol _ | MarkedSymbol _ => true
+      | _ => false
+      end.
+
+    Definition M2 x :pTM sig__M bool 1 := if negb (Option.apply (@isMarked sig) false x)
                                  then Return Nop false
                                  else
-                                   MoveToSymbol (fun x => isMarked x || isLeftBorder x || isRightBorder x) id;;
-                                   Relabel ReadChar (Option.apply isRightBorder false).
+                                   MoveToSymbol (fun x => isMarked x || isLeftBlank x || isRightBlank x || isNilBlank x) id;;
+                                   Relabel ReadChar (Option.apply isRightBlank false).
+
+    Definition f__M2 x t : (bool*tape sig__M) :=
+      if negb (Option.apply (@isMarked sig) false x)
+      then (false,t)
+      else let t' := MoveToSymbol_Fun (fun x => isMarked x || isLeftBlank x || isRightBlank x) id t in
+           (Option.apply isRightBlank false (current t'),t').
 
     Definition caseFirstSymbol : pTM sig__M (bool+bool) 1:=
       Switch
@@ -88,17 +109,262 @@ Module CheckEncodesTape.
            | _ => Return Nop (inl false)
            end).
 
+    Definition f__caseFirstSymbol (t: tape sig__M): (bool+bool):=
+      match current t with
+        Some NilBlank => inl true
+      | Some (LeftBlank b) => inr b
+      | _ => inl false
+      end.
+
+    Definition M__step : bool*bool -> pTM sig__M ((bool*bool) + bool) 1 :=
+      fun '(haveSeenMark,haveSeenSymbol) =>
+        Switch
+          ReadChar
+          (fun x =>
+             match x with
+               None => Return Nop (inr false)
+             | Some c =>
+               if (isMarked c && haveSeenMark) || isNilBlank c || isLeftBlank c || isRightBlank c
+               then Return Nop (inr (isRightBlank c && negb (haveSeenMark || isMarked c)))
+               else Return (Move R) (inl (haveSeenMark || isMarked c,haveSeenSymbol || isSymbol c))
+             end).
+
+    Definition f__step bs t : (bool * bool + bool) * tape sig__M :=
+      let (haveSeenMark,haveSeenSymbol) := (fst bs,snd bs) in
+      match current t with
+        None => (inr false,t)
+      | Some c =>
+        if (isMarked c && haveSeenMark) || isNilBlank c || isLeftBlank c || isRightBlank c
+        then (inr (isRightBlank c && (xorb haveSeenMark (isMarked c)) && haveSeenSymbol),t)
+        else (inl (haveSeenMark || isMarked c,haveSeenSymbol || isSymbol c),tape_move_right t)
+      end.
+
+    Definition M' (bs : bool*bool) := 
+      StateWhile M__step bs.
+
+    Function f' bs t { measure rlength t } : (bool * tape sig__M)  :=
+      let r := f__step bs t in
+      match fst r with 
+        inl bs' => f' bs' (snd r)
+      | inr b => (b,(snd r))
+      end.
+    Proof.
+      unfold f__step. intros [haveSeenMark haveSeenSymbol] [ | | | ? c t__R] ?;cbn.
+      1-3:now intros [=].
+      destruct c as [ [] | [] | | | ];cbn. all:try solve [inversion 1].
+      1-4:destruct haveSeenMark;cbn.
+      all:intros [= <-]. all:destruct t__R;cbn. all:nia.
+    Qed.
+    
     Definition M : pTM sig__M bool 1:=
-      Switch caseFirstSymbol
-             (fun x =>
-                match x with
-                  inl b => Return Nop b
-                | inr b =>
-                  (if b then Nop
-                   else Move R);;
-                  MoveToSymbol (fun x => isMarked x || isLeftBorder x || isRightBorder x) id;;
-                  Switch ReadChar M2
-                end).
+      If (Relabel ReadChar (Option.apply isLeftBlank false))
+         (Switch ReadChar (fun c => Move R;; M' (Option.apply (@isMarked _) false c,false)))
+         (Relabel ReadChar (Option.apply isNilBlank false)).
+
+    Definition f (t : tape sig__M) : (bool*tape sig__M) :=
+      match current t with
+        None => (false,t)
+      | Some c =>
+        if isLeftBlank c then  f' (isMarked c,false) t
+        else (isNilBlank c, t)
+      end.
+
+    Lemma encode_tape_invariants x b t t__R:
+         encode_tape x = LeftBlank b :: t ++t__R
+         -> (forall x, x el t  -> isSymbol x = true)
+         -> t__R <> []
+           /\ (forall c : sig__M , c el tail (rev t__R) -> isSymbol c = true)
+           /\ (exists b', head (rev t__R) = Some (RightBlank b'))
+           /\ (length (filter (@isMarked _) (t__R++t++[LeftBlank b])) = 1)
+           /\ length (t++t__R) > 1.
+    Proof using sig.
+    Admitted.
+
+    Lemma invert_symbols_0_marked (t: list sig__M):
+      length (filter (@isMarked _) t ) = 0
+      -> (forall x : sigTape (eqType_X (type sig)), x el t -> isSymbol x = true)
+      -> exists s : list sig, t = map UnmarkedSymbol s.
+    Proof.
+      induction t. now eexists [].
+      cbn. intros H1 H2. destruct a eqn:H';cbn in *.
+      1,2,3:now specialize (H2 a);subst a;discriminate H2.
+      -nia.
+      -edestruct IHt as (?&->). 3:now eexists (_::_). all:easy.
+    Qed.
+
+    Lemma invert_symbols_1_marked (t: list sig__M):
+      length (filter (@isMarked _) t ) = 1
+      -> (forall x : sigTape (eqType_X (type sig)), x el t -> isSymbol x = true)
+      -> exists s1 c (s2 : list sig), t = map UnmarkedSymbol s1 ++ (MarkedSymbol c :: map UnmarkedSymbol s2).
+    Proof.
+      induction t. now inversion 1.
+      cbn. intros H1 H2. destruct a eqn:H';cbn in *.
+      1,2,3:now specialize (H2 a);subst a;discriminate H2.
+      -edestruct invert_symbols_0_marked with (t:=t) as (?&->).  1,2:easy.
+       eexists [],_,_. reflexivity.
+      -edestruct IHt as (?&?&?&->). 3:now eexists (_::_),_,_. all:easy.
+    Qed.
+
+    Ltac length_not_nil :=
+      let H := fresh "H" in
+      intros H; apply (f_equal (@length _)) in H;repeat (try autorewrite with list in H;cbn in H);nia.
+
+    Local Hint Rewrite filter_app : list. 
+
+    Lemma filter_rev (A : Type) (f : A -> bool) (l : list A): filter f (rev l) = rev (filter f l).
+    Proof.
+      induction l;cbn in *. easy. autorewrite with list. cbn;destruct f. all:cbn;try now autorewrite with list.
+    Qed.
+
+    Local Hint Rewrite filter_rev : list. 
+
+    Lemma f'_spec (seenMark seenSymbol : bool) t__L' b t__L c t__R res:
+      (length (filter (@isMarked _) (t__L'++[LeftBlank b])) = if seenMark then 1 else 0)
+      -> (forall x, x el t__L' -> isSymbol x = true)
+      -> reflect (t__L' <> []) seenSymbol
+      -> res =  f' (seenMark,seenSymbol) (midtape (t__L'++LeftBlank b::t__L) c t__R)
+      ->  if fst res then
+          exists (x:tape sig) (t__R1 t__R2 : list sig__M),
+          t__R = t__R1++t__R2
+          /\ encode_tape x = LeftBlank b :: rev t__L'++c::t__R1
+          /\ snd res = midtape (tail (rev t__R1++[c])++t__L'++LeftBlank b::t__L) (hd c (rev t__R1)) t__R2
+        else
+          forall x (t__R1 t__R2 : list sig__M),
+          t__R = t__R1++t__R2 -> 
+            encode_tape x <> LeftBlank b :: rev t__L'++c::t__R1
+        .
+    Proof.
+      remember (length t__R) as n0 eqn: Hn0. revert t__R Hn0 t__L' c res seenMark seenSymbol.
+      induction n0 as [n0 IH] using lt_wf_ind. intros ? -> ? ? res ? ?;cbn in *.
+      intros H__seenMark H__symbs H__seenSymbol Hres. 
+      rewrite f'_equation in Hres.
+      destruct c;cbn. 1-3:clear IH.
+      -replace (res.1) with false.
+       2:{ cbn in Hres. destruct marked;cbn in Hres. destruct seenMark in Hres;cbn in Hres. all:now subst. }
+       clear - H__symbs.
+       intros ? ? ? -> (Hneq&Hsym&(?&Hlast)&_)%encode_tape_invariants;cbn in *. 2:now setoid_rewrite <- in_rev.
+       destruct t__R1. easy. discriminate (Hsym (LeftBlank marked)). rewrite tl_app. 2:now length_not_nil. now cbn.     
+      -revert Hres. cbn. rewrite !orb_true_r.
+       destruct marked;cbn in *. destruct seenMark;cbn in *. all:intros ->;cbn. 3:destruct seenMark;cbn. 2,3:destruct seenSymbol;cbn.
+       +intros ? ? ? -> (Hneq&Hsym&(?&Hlast)&Hmarks)%encode_tape_invariants;cbn in *. 2:now setoid_rewrite <- in_rev.
+        autorewrite with list in *. nia.
+       +edestruct invert_symbols_0_marked with (t:= t__L') as (t__R2&->).
+        1,2:autorewrite with list in *. now nia. now intros;eapply H__symbs.
+        destruct b. 1:{exfalso. autorewrite with list in H__seenMark. now cbn in H__seenMark. } 
+        destruct t__R2 as [ | c' cs] eqn:Htp. 1:{exfalso. inversion H__seenSymbol. easy. } 
+        eexists (rightof _ _),[],_. repeat eapply conj. 1,3:reflexivity. cbn.
+        autorewrite with list;cbn.  setoid_rewrite <- map_rev with (l:=cs) at 2. easy.
+       +intros ? ? ? -> (Hneq&Hsym&(?&Hlast)&Hmarks&Hnempty)%encode_tape_invariants;cbn in *. 2:now setoid_rewrite <- in_rev.
+        destruct t__L'. all:inv H__seenSymbol. 2:now apply H. cbn in *;autorewrite with list in *.
+        destruct t__R1. 2:{ ediscriminate (Hsym (RightBlank _)). rewrite tl_app. eauto. length_not_nil. }
+        cbn in *. nia.
+       +destruct b.
+        *edestruct invert_symbols_0_marked with (t:= t__L') as (t__R2&->).
+         1,2:autorewrite with list in *;cbn in *. now nia. now intros;eapply H__symbs.
+         destruct t__R2 eqn:?. 1:{exfalso. inversion H__seenSymbol. easy. }
+         destruct (rev t__R2) eqn:Htp. 1:{exfalso. subst. revert Htp. length_not_nil. } 
+         eexists (leftof _ _),[],_. repeat eapply conj. 1,3:reflexivity. rewrite <- Heql. cbn.
+         autorewrite with list;cbn.  setoid_rewrite <- map_rev with (l:=t__R2). now rewrite Htp.
+        *edestruct invert_symbols_1_marked with (t:= t__L') as (?&?&?&->).
+         1,2:autorewrite with list in *;cbn in *. now nia. now intros;eapply H__symbs.
+         eexists (midtape _ _ _),[],_. repeat eapply conj. 1,3:reflexivity. cbn.
+         repeat (autorewrite with list;cbn).  setoid_rewrite map_rev. easy.
+       +intros ? ? ? -> (Hneq&Hsym&(?&Hlast)&Hmarks&?)%encode_tape_invariants;cbn in *. 2:now setoid_rewrite <- in_rev.
+        destruct t__R1. 2:{ ediscriminate (Hsym (RightBlank _)). rewrite tl_app. 2:now length_not_nil. easy. }
+        destruct t__L'. 2:{ inversion H__seenSymbol. now apply H0. }
+        cbn in *. nia.
+       +intros ? ? ? -> (Hneq&Hsym&(?&Hlast)&Hmarks&?)%encode_tape_invariants;cbn in *. 2:now setoid_rewrite <- in_rev.
+        destruct t__R1. 2:{ ediscriminate (Hsym (RightBlank _)). rewrite tl_app. 2:now length_not_nil. easy. }
+        cbn in *. autorewrite with list in *. nia.
+      -replace (res.1) with false.
+       2:{ cbn in Hres. destruct seenMark in Hres;cbn in Hres. all:now subst. }
+       clear - H__symbs.
+       intros ? ? ? -> (Hneq&Hsym&(?&Hlast)&_)%encode_tape_invariants;cbn in *. 2:now setoid_rewrite <- in_rev.
+       destruct t__R1. easy. discriminate (Hsym (NilBlank)). rewrite tl_app. 2:now length_not_nil. now cbn.   
+      -revert Hres. cbn. destruct seenMark;cbn.
+       {clear IH. intros ->;cbn.
+        intros ? ? ? -> (Hneq&Hsym&(?&Hlast)&?&?)%encode_tape_invariants;cbn in *. 2:now setoid_rewrite <- in_rev.
+        cbn in *. autorewrite with list in *. nia.
+       }
+       destruct t__R.
+       { clear IH. cbn. rewrite f'_equation;cbn.  
+         intros ->;cbn.
+         intros ? ? ? Hnil (Hneq&Hsym&(?&Hlast)&?&?)%encode_tape_invariants;cbn in *. 2:now setoid_rewrite <- in_rev.
+         destruct t__R1. 2:easy. destruct t__R2. 2:easy. easy.
+       }
+       cbn. intros H.
+       autorewrite with list in H__seenMark. destruct b;cbn in H__seenMark. easy. 
+       specialize IH with (t__L' := MarkedSymbol s :: t__L');cbn in IH. eapply IH in H;clear IH.
+       3:reflexivity. 2:easy. 2:now autorewrite with list in *;nia. 2:now intros ? [<- | ];easy.
+       2:now rewrite orb_true_r;constructor.
+       
+        
+      -admit.
+    Qed.
+            
+       intros [] ? Hx;cbn in Hx.
+      cbn in *. 
+      all:cbn.
+      induction size_induction with (f )
+      induction t__R in t__L',c
+      cbv beta delta [f__M Rel ContainsEncoding
+                         ng.Rel].
+      destruct f__caseFirstSymbol eqn:case1.
+      {intros [= -> <-];revert case1. destruct t as [ | | | ? [] ?] eqn:Ht;cbn;intros [= <-].
+        1-3:easy.
+        2:now eexists (@niltape _),_,_.
+        all:now intros ? [] ?;cbn.
+      }
+      set (t1 := if b0 then t else tape_move_right t). cbn.
+      destruct (MoveToSymbol_Fun_is_rel (fun x : sigTape (eqType_X (type sig)) => isMarked x || isLeftBorder x || isRightBorder x)
+                                        (@id _) t1) as [H'|H'].
+      all: set (t2 := MoveToSymbol_Fun _ _ _);cbn in *;fold t2 in H'. 
+
+      { destruct H' as (H'&<-). setoid_rewrite H'. cbn.
+        intros [= <- <-]. destruct t as [ | | | ? c ?] eqn:Ht;cbn. 1-3:easy.
+        subst t1;destruct b0. easy.
+        cbn in *. destruct c;inv case1. destruct l0;inv H'. intros ? [] ?.
+        all:cbn;intros [= <-  Hnil]. all: eapply in_nil;rewrite Hnil. all:eauto.
+      }
+      destruct H' as (t__L&c&t__R1&t__R2&Ht1&Hall1&Hc&H'). subst t1. 
+      destruct H' as [ -> | [-> ->]]. all:cbn in *.
+      2:{
+        assert (Hall : forall x, x el (c :: t__R1) -> isMarked x || isLeftBorder x || isRightBorder x = false).
+        {intros x. rewrite app_removelast_last at 1. 2:easy.
+         intros [ | [<- | []]]%in_app_or. all:easy.
+        } clear Hall1 Hc.
+        intros [= <- <-]. rewrite app_nil_r in Ht1. destruct t as [ | | | ? c' ?];cbn. 1-3:easy. 
+          (destruct c';revert case1;intros [= <-]);[]. 
+          intros ? x ?. destruct x eqn:Hx;intros [= -> -> ->]. autorewrite with list in *.
+          all:inv Ht1.
+        -now discriminate (Hall (LeftBlank true)).
+        -destruct rev. all:cbn in *. all:inv H0.
+         +now discriminate (Hall (RightBlank true)).
+         +discriminate (Hall (RightBlank true)). autorewrite with list;cbn. eauto.
+        -destruct rev. all:cbn in *. all:inv H0.
+         +discriminate (Hall (RightBlank false)). autorewrite with list;cbn. eauto.
+         +discriminate (Hall (RightBlank false)). repeat (autorewrite with list;cbn). eauto 10.
+      }
+      unfold f__M2. cbn. destruct isMarked. all:cbn.
+      2:{ cbn in *.
+          intros [= <- <-]. destruct t as [ | | | ? c' ?];cbn. 1-3:easy. cbn in *. 
+          (destruct c';revert case1;intros [= <-]);[]. 
+          intros ? x ?. destruct x eqn:Hx;intros [= -> -> ->]. autorewrite with list in *.
+          -revert Ht1;intros [= -> <- Ht__R].
+           destruct t__R1;cbn in *.
+        -now discriminate (Hall (LeftBlank true)).
+        -destruct rev. all:cbn in *. all:inv H0.
+         +now discriminate (Hall (RightBlank true)).
+         +discriminate (Hall (RightBlank true)). autorewrite with list;cbn. eauto.
+        -destruct rev. all:cbn in *. all:inv H0.
+         +discriminate (Hall (RightBlank false)). autorewrite with list;cbn. eauto.
+         +discriminate (Hall (RightBlank false)). repeat (autorewrite with list;cbn). eauto 10.
+      cbn. 
+         +inv H0. destruct t__R;cbn in *. all:cbn in *;autorewrite with list in *.
+            *rewrite <- hd_rev in *. cbn in *. autorewrite with list in *. now cbn in *.
+            *rewrite removelast_as_tail in Hall1. repeat
+    
+    
 
 
     (** Verification*)
@@ -137,77 +403,263 @@ Module CheckEncodesTape.
         tacInEvar R (destruct g as P);destruct g as P;cbn zeta iota
       end.
 
-    Lemma Realises : M ⊨ Rel.
+    (* MOVE *)
+    Lemma last_not_default X (d d':X) A :
+      A <> [] -> last A d = last A d'.
+    Proof. induction A. easy. destruct A;cbn. easy. intros ?. now apply IHA. Qed.
+
+    (*MOVE *)
+
+    Definition MoveToSymbol_Rel_nice (sig':finType) (f:sig' -> bool) (g:sig' -> sig') t t' := 
+      ((current t = None /\ t = t')
+         \/ (exists t__L c t__R1 t__R2,
+               t = midtape t__L c (t__R1++t__R2)
+               /\ (forall x, x el (removelast (c::t__R1)) -> f x = false)
+               /\ f (last (c::t__R1) c) = ssrbool.isSome (current t')
+               /\ (t' = midtape (rev (map g (removelast (c::t__R1)))++t__L) (g (last (c::t__R1) c)) t__R2
+                  \/ (t' = rightof (g (last (c::t__R1) c)) (rev (map g (removelast (c::t__R1)))++t__L) /\ t__R2 = [])))).
+    
+    Lemma MoveToSymbol_Fun_nice (sig':finType) (f:sig' -> bool) (g:sig' -> sig') t t' :
+      MoveToSymbol_Fun f g t = t' <-> MoveToSymbol_Rel_nice f g t t'. 
+    Proof.
+      Local Arguments removelast : simpl nomatch.
+      Local Arguments last : simpl nomatch.
+      clear n.
+      remember (tape_local t) as A eqn:eqA.
+      revert t t' eqA. unfold MoveToSymbol_Rel_nice.
+      induction A using (size_induction (f:=@length sig'));intros t t' eqA.
+      rewrite MoveToSymbol_Fun_equation. destruct current eqn:eq.
+      2:{ split. now left. intros [ | H']. easy. destruct H' as (?&?&?&?&->&?). easy. }
+      destruct f eqn:Hf.
+      { destruct t;inv eq. all:cbn. split.
+        -intros <-. right. eexists _,_,[],_.
+         repeat split;now cbn.
+        -intros [ | (t__L&c&t__R1&t__R2&[= -> -> -> ]&Hfalse&Hc&H'')];[ easy | ].
+         destruct t__R1 as [ | c__R t__R1].
+         2:{exfalso. cbn in *. rewrite Hfalse in Hf;easy. }
+         cbn in *. 
+         destruct H'' as [-> | [-> -> ]]. all:cbn in *;easy.
+      }
+      destruct t. all:inv eq. destruct l0. all:cbn - [removelast].
+      all:rewrite H;[ | | reflexivity];[cbn | cbn;nia].
+      - cbn. split.
+        +intros [(_&<-)| (?&?&?&?&[=]&?)];[]. right.
+         eexists _,_,[],[]. split;[reflexivity| ]. split;[easy| ]. unfold last, removelast;cbn. easy.
+        +intros [([=]&?)|(t__L&c&t__R1&t__R2&[= <- <- H__nil]&Hfalse&Hc&H'')];[].
+         destruct t__R1;[ |now inv H__nil]. destruct t__R2;[ |now inv H__nil]. clear H__nil.
+         cbn in H''|-*. destruct H'' as [-> | [-> _ ]]. 2:now left. now unfold last in Hc;cbn in Hc.
+      -eapply Morphisms_Prop.or_iff_morphism. easy.
+       split. all:intros (t__L&c&t__R1&t__R2&Heq&Hfalse&Hc&H');revert Heq.
+       +intros [= <- -> ->]. eexists _,_,(_::_),_. split. reflexivity.
+        cbn. split. now intros ? [-> | ].
+        autorewrite with list in |-*;cbn. erewrite last_not_default. split;easy. easy.
+       +intros [= -> -> Heq]. destruct t__R1.
+        {cbn in *. destruct H' as [ -> | [-> ->]]. all: now cbn in *. }
+        revert Heq;intros [= -> ->].
+        eexists (_::_),_,_,_. split. reflexivity. cbn in *.
+        split. easy. autorewrite with list in H';cbn. erewrite last_not_default. 2:easy. split;easy.
+    Qed.
+
+    Lemma MoveToSymbol_Fun_is_rel (sig':finType) (f:sig' -> bool) (g:sig' -> sig') t :
+      MoveToSymbol_Rel_nice f g t (MoveToSymbol_Fun f g t).
+    Proof.
+      now rewrite <- MoveToSymbol_Fun_nice.
+    Qed.
+
+    (* MOVE *)
+    Lemma removelast_as_tail X (x:list X): removelast x = rev (tail (rev x)).
+    Proof.
+      rewrite tl_rev. now autorewrite with list.
+    Qed.
+    
+    Lemma Realises : M ⊨ (fun tin '(b,tout) => f__M tin[@Fin0] = (b,tout[@Fin0])).
     Proof.
       eapply Realise_monotone.
-      { unfold M. apply Switch_Realise
-                    with (R1 :=
-                            fun tin '(yout, tout) =>
-                              tin = tout /\
-                              match yout with
-                                inl true => current tin[@Fin0] = Some NilBlank
-                              | inr b => current tin[@Fin0] = Some (LeftBlank b)
-                              | inl false => (forall b, current tin[@Fin0] <> Some (LeftBlank b)) /\ current tin[@Fin0] <> Some NilBlank
-                              end).
-        { eapply Realise_monotone.
+      { unfold M. eapply Switch_Realise with (R1:=fun t '(b,t') => f__caseFirstSymbol t[@Fin0] = b /\ t=t').
+        { eapply Realise_monotone. 
           {unfold caseFirstSymbol. TM_Correct. }
-          hnf;cbn. intros t0 [y1 t1]. intros (?&?&[-> ->]&H__cur).
-          repeat destruct _ in H__cur. all:revert H__cur;cbn. all:intros (->&_&->).
-          all:split;[easy| ]. all:intuition congruence.
+          hnf;cbn. intros t0 [y1 t1]. intros (?&?&[-> ->]&H__cur). unfold f__caseFirstSymbol.
+          destruct t0[@Fin0] as [ | | | t__L [ [] | [] | | | ] t__R] eqn:Ht0;cbn in H__cur|-*. all:revert H__cur. all:cbn;intros (->&?&->).
+          all:split;congruence.
         }
-
         introsSwitch [[]| b]. 1,2:now cbn;refine (Return_Realise _); TM_Correct.
         eapply Seq_Realise. 1:now destructBoth b as []; TM_Correct.
         TM_Correct_step. now TM_Correct.
-
+        
         apply Switch_Realise. now TM_Correct.
         unfold M2;cbn. introsSwitch opt.
         destructBoth (negb (oapp (isMarked (sig:=eqType_X (type sig))) false opt)) as []. TM_Correct. TM_Correct.
       }
-      unfold Rel,ContainsEncoding.Rel. hnf;cbn.
+      cbv delta [f__M] beta. intros t0 (l1&t1). intros (read1&?&(<-&<-)&H');revert H'.
+      destruct (f__caseFirstSymbol t0[@Fin0]) as [[]| ];cbn beta delta. 1,2:now intros (?&?&?);congruence.
+      intros (f&t2&Ht0&?&t3&Ht3&HH&?&(->&->)&H'). cbn beta delta iota in *. 
+      set (t2':=if b then t0[@Fin0] else tape_move_right t0[@Fin0]).
+      set (t3' := MoveToSymbol_Fun
+       (fun x0 : eqType_X (type (finType_CS (sigTape (eqType_X (type sig))))) =>
+          isMarked x0 || isLeftBorder x0 || isRightBorder x0) id t2'). cbn in *.
+      replace t2 with [|t2'|] in *.
+      2:{apply Vector.eq_nth_iff. intros i ? <-. rewrite (StepTM.finSucc_help i);cbn.
+         destruct b;cbn in Ht0. all:now subst t2'; setoid_rewrite <- Ht0. } clear t2 Ht0. cbn in *. 
+      replace t3 with [|t3'|] in *.
+      2:{apply Vector.eq_nth_iff. intros i ? <-. rewrite (StepTM.finSucc_help i);cbn.
+         rewrite Ht3;subst t3'. easy. } clear t3 Ht3. fold t3'.
+      unfold f__M2. cbn in *.
+      destruct negb eqn:Htmp. 1:now destruct H' as (->&_&->).
+      cbn in H'. destruct H' as (_&?&Ht4&?&->&->&<-);rewrite Ht4 in *. reflexivity.
+    Qed.
+
+    Lemma Rel_if t b t': f__M t = (b,t') -> Rel [|t|] (b,([|t'|])).
+    Proof.
+      cbv beta delta [f__M Rel ContainsEncoding.Rel].
+      destruct f__caseFirstSymbol eqn:case1.
+      {intros [= -> <-];revert case1. destruct t as [ | | | ? [] ?] eqn:Ht;cbn;intros [= <-].
+        1-3:easy.
+        2:now eexists (@niltape _),_,_.
+        all:now intros ? [] ?;cbn.
+      }
+      set (t1 := if b0 then t else tape_move_right t). cbn.
+      destruct (MoveToSymbol_Fun_is_rel (fun x : sigTape (eqType_X (type sig)) => isMarked x || isLeftBorder x || isRightBorder x)
+                                        (@id _) t1) as [H'|H'].
+      all: set (t2 := MoveToSymbol_Fun _ _ _);cbn in *;fold t2 in H'. 
+
+      { destruct H' as (H'&<-). setoid_rewrite H'. cbn.
+        intros [= <- <-]. destruct t as [ | | | ? c ?] eqn:Ht;cbn. 1-3:easy.
+        subst t1;destruct b0. easy.
+        cbn in *. destruct c;inv case1. destruct l0;inv H'. intros ? [] ?.
+        all:cbn;intros [= <-  Hnil]. all: eapply in_nil;rewrite Hnil. all:eauto.
+      }
+      destruct H' as (t__L&c&t__R1&t__R2&Ht1&Hall1&Hc&H'). subst t1. 
+      destruct H' as [ -> | [-> ->]]. all:cbn in *.
+      2:{
+        assert (Hall : forall x, x el (c :: t__R1) -> isMarked x || isLeftBorder x || isRightBorder x = false).
+        {intros x. rewrite app_removelast_last at 1. 2:easy.
+         intros [ | [<- | []]]%in_app_or. all:easy.
+        } clear Hall1 Hc.
+        intros [= <- <-]. rewrite app_nil_r in Ht1. destruct t as [ | | | ? c' ?];cbn. 1-3:easy. 
+          (destruct c';revert case1;intros [= <-]);[]. 
+          intros ? x ?. destruct x eqn:Hx;intros [= -> -> ->]. autorewrite with list in *.
+          all:inv Ht1.
+        -now discriminate (Hall (LeftBlank true)).
+        -destruct rev. all:cbn in *. all:inv H0.
+         +now discriminate (Hall (RightBlank true)).
+         +discriminate (Hall (RightBlank true)). autorewrite with list;cbn. eauto.
+        -destruct rev. all:cbn in *. all:inv H0.
+         +discriminate (Hall (RightBlank false)). autorewrite with list;cbn. eauto.
+         +discriminate (Hall (RightBlank false)). repeat (autorewrite with list;cbn). eauto 10.
+      }
+      unfold f__M2. cbn. destruct isMarked. all:cbn.
+      2:{ cbn in *.
+          intros [= <- <-]. destruct t as [ | | | ? c' ?];cbn. 1-3:easy. cbn in *. 
+          (destruct c';revert case1;intros [= <-]);[]. 
+          intros ? x ?. destruct x eqn:Hx;intros [= -> -> ->]. autorewrite with list in *.
+          -revert Ht1;intros [= -> <- Ht__R].
+           destruct t__R1;cbn in *.
+        -now discriminate (Hall (LeftBlank true)).
+        -destruct rev. all:cbn in *. all:inv H0.
+         +now discriminate (Hall (RightBlank true)).
+         +discriminate (Hall (RightBlank true)). autorewrite with list;cbn. eauto.
+        -destruct rev. all:cbn in *. all:inv H0.
+         +discriminate (Hall (RightBlank false)). autorewrite with list;cbn. eauto.
+         +discriminate (Hall (RightBlank false)). repeat (autorewrite with list;cbn). eauto 10.
+      cbn. 
+         +inv H0. destruct t__R;cbn in *. all:cbn in *;autorewrite with list in *.
+            *rewrite <- hd_rev in *. cbn in *. autorewrite with list in *. now cbn in *.
+            *rewrite removelast_as_tail in Hall1. repeat (cbn in Hall1;autorewrite with list in Hall1).
+             destruct t__R;cbn in *.
+             
+             idtac. 
+             destruct MoveToSymbol_Fun eqn:Hmv1.
+             unfold f__M2;destruct t1;cbn.
+             unfold f__M2.
+             set (t2:=MoveToSymbol_Fun
+                        (fun x : eqType_X (type (finType_CS (sigTape (eqType_X (type sig))))) => isMarked x || isLeftBorder x || isRightBorder x)
+                        id t2).
+          -destruct b.
+        +intros (?&?&?&->&->);revert case1;cbn. destruct x;intros [= <-]. reflexivity.
+        +revert case1. destruct t as [ | | | ? [] ?] eqn:Ht;cbn. all:intros [= <-]. destructintros H. destrdestruct c;inv H
+      cbn.
+         destruct b;cbn in Ht0. all:now subst t2'; setoid_rewrite <- Ht0. } clear t2 Ht0.
+         -
+ intros 
+      
+
+
+      
+      unfold Rel,ContainsEncoding.Rel. hnf;cbn in *.
       intros t0 (l1&t1). intros (read1&?&(<-&?)&H');revert H'. destruct read1 as [[]| ];cbn.
       -intros (->&_&->). destruct t0[@Fin0];inv H.
        eexists (@niltape sig),_,_. repeat split.
       -intros (->&_&->). intros ? [] ?;destruct t0[@Fin0];cbn in H|-*;easy.
-      -intros ([]&t2&Ht2&_&t3&Ht3&?&?&[-> ->]&H');revert H'.
+      -destruct t0[@Fin0] eqn:Ht0; inv H.
+       intros ([]&t2&Ht2&_&t3&Ht3&?&?&[-> ->]&H');revert H'.
+       symmetry in Ht3. apply MoveToSymbol_Fun_spec in Ht3. cbn in Ht3. setoid_rewrite map_id in Ht3.
+       destruct Ht3 as [(Ht2'&<-) | (t__L&c&t__R1&t__R2&Ht2'&Hfalse&Hc&Ht3)].
+       { rewrite Ht2'. cbn. intros (->&?&<-). intros ? x0 ? [= -> Hneq ->].
+         destruct x0;inv Hneq;cbn in Ht2.
+         -subst t2. now rewrite Ht0 in Ht2'.
+         -rewrite Ht2 in Ht2'. rewrite Ht0 in Ht2';cbn in Ht2'.
+          destruct (rev l) eqn:Hl; cbn in Ht2'. all:easy.
+         -rewrite Ht2 in Ht2'. rewrite Ht0 in Ht2';cbn in Ht2'.
+          destruct (rev l) eqn:Hl; cbn in Ht2'. all:easy.
+       }
+       destruct Ht3 as [Ht3 | (Ht3&->)]. all:rewrite Ht3;cbn.
+       2:{ intros (->&_&<-). intros ? x0 ? [= -> Hneq ->].
+           rewrite Ht3 in Hc;cbn in Hc.
+           destruct x0;inv Hneq;cbn in Ht2.
+           -subst t2. rewrite Ht0 in Ht2'. inv Ht2'.
+            destruct t__R1.
+            2:{ specialize Hfalse with (LeftBlank true). discriminate Hfalse. now cbn. }
+            now discriminate H2.
+           -rewrite Ht0 in Ht2. rewrite Ht2 in Ht2';inv Ht2'. rewrite app_nil_r in H0.  clear t0 Ht0. clear t2 Ht2. clear t1 Ht3. clear - Hfalse Hc H0.
+            destruct (rev l) eqn:Hl; cbn in H0. all:inv H0;cbn in *. destruct t__R;cbn in *. all:try easy.
+            +now specialize (Hfalse (RightBlank true)).
+            +autorewrite with list in *;cbn in *.
+             
+             Ltac length_not_nil :=
+               let H := fresh "H" in
+               intros H; apply (f_equal (@length _)) in H;repeat (try autorewrite with list in H;cbn in H);nia.
+             rewrite StepTM.removelast_cons in Hfalse. 2:length_not_nil. 
+             rewrite removelast_app in Hfalse. 2:easy. cbn [removelast] in Hfalse.
+             
+             
+             (*TODO: last: app and cons rules in Hc. *)
+             
+             2:{ 
+             erewrite (removelast_app (UnmarkedSymbol e0 :: map UnmarkedSymbol l0)) in Hfalse.
+            + destruct t__R1. all:inv H3. cbn in *.
+              specialize (Hfalse with  term+)
+              apply Hfalse. easy.
+            
+         -rewrite Ht2 in Ht2'. rewrite Ht0 in Ht2';cbn in Ht2'.
+          destruct (rev l) eqn:Hl; cbn in Ht2'. all:easy.
+         -rewrite Ht2 in Ht2'. rewrite Ht0 in Ht2';cbn in Ht2'.
+          destruct (rev l) eqn:Hl; cbn in Ht2'. all:easy.
+       destruct oapp eqn:Hb;cbn.
+       2:{ intros (->&?&<-);cbn.
+           destruct Ht3 as [Ht1 | (Ht1 & ->)].
+           -rewrite Ht1 in Hb,Hc;cbn in Hb,Hc. rewrite Hb in Hc. cbn in Hc.
+            rewrite cbn in 
+           destruct (current t1[@Fin0]) eqn:Ht1. cbn in Hb,Hc.
+           destruct (last (c :: t__R1) c) eqn: Hl;cbn in Hc,Ht3.  destruct t0[@Fin0] eqn:eqt0;inv H. destruct b;cbn in Ht2.
+           {subst t2. rewrite eqt0 in *. inv Ht2'. erewrite MoveToSymbol_Step_Fun_M2_true in Ht3. 2,3:reflexivity.
+            cbn in Ht3. rewrite Ht3 in Hb. now cbn in Hb.
+           }
+           rewrite eqt0 in Ht2.
+           destruct l0;cbn in Ht2.
+           rewrite Ht2 in Ht3. cbn in *. 
+           
+            rewrite MoveToSymbol_Fun_equation in Ht3lcbn in   in Ht3. cbn in Ht3. now  rewrite eqt0 in Ht2'. }
+         rewrite eqt0 in Ht2. cbn in Ht2. rewrite Ht2 in Ht2'. destruct l0;cbn in Ht2,Ht2';inv Ht2'.
+         intros ? x0 ? [= ->]. symmetry in H1;apply appendNil in H1 as [H1 ->].
+         destruct x0. all:cbn in H1;try easy. all:eapply in_nil;rewrite <- H1. all:easy.
+
+       destruct (current t3[@Fin0]) eqn: Hct3. c
+       2:{ cbn. 
        (*destruct (current t3[@Fin0]) eqn:H__cur;cbn.
        2:{intros (->&?&<-). destruct b;cbn in Ht2.
           - subst t2. destruct t1[@Fin0];cbn in *;try easy. *)
 
-       Lemma MoveToSymbol_id_spec (f:sig -> bool) t t' :
-         MoveToSymbol_Fun f id t = t' <-> ((current t = None /\ t = t')
-                                        \/ (exists t__L c t__R1 t__R2,
-                                              t = midtape t__L c (t__R1++t__R2)
-                                              /\ (forall x, x el removelast (c::t__R1) -> f x = false)
-                                              /\ tape_local_l t' = (rev (c::t__R1)++t__L)
-                                              /\ right t' = t__R2)). 
-       Proof.
-         clear n M2.
-         remember (tape_local t) as A eqn:eqA.
-         revert t t' eqA.
-         induction A using (size_induction (f:=@length sig));intros t t' eqA.
-         rewrite MoveToSymbol_Fun_equation. destruct current eqn:eq.
-         2:{ split. now left. intros [ | H']. easy. destruct H' as (?&?&?&?&->&?). easy. }
-         destruct f eqn:Hf.
-         { destruct t;inv eq. all:cbn. split.
-           -intros <-. right. eexists _,_,[],_.
-            repeat split. now intros ? [].
-           -intros [ | (?&?&?&?&[= -> -> -> ]&Hann&H''&<-)];[ easy | ].
-            destruct t';cbn in H''|-*. all:autorewrite with list in *.
-            all:try solve [apply (f_equal (@length _)) in H'';repeat (cbn in H'';autorewrite with list in H'');nia].
-            destruct x1. 2:{ exfalso. erewrite Hann in Hf. all:easy. }  cbn in *. congruence.
-         }
-         destruct t. all:inv eq. destruct l0. all:cbn - [removelast].
-         all:rewrite H;[ | | reflexivity];[ | cbn;nia].
-         - Fail. cbn. 
-         -
-           all:cbn cbn [doAct]. 
-                               +destruct l0. 2:easy. ccbn. subst. congruence. 2:rewrite <- H0;cbn.  2:split. intuition. easy. split. 
-         split.
-         2:{ intros [[H <-] | H].
-             -rewrite MoveToSymbol_Step_Fun_M2_None. 2:easy. unfold MoveToSymbol_Step_Fun. now rewrite H.
-             -destruct H as (?&?&?&?&->&Hall&Hleft&Hright).
-              erewrite MoveToSymbol_correct.
+       
          (* MoveToSymbol_correct:
   forall (sig : finType) (stop : eqType_X (type sig) -> bool) (f : eqType_X (type sig) -> eqType_X (type sig))
     (t : tape (eqType_X (type sig))) (str1 str2 : list (eqType_X (type sig))) (x : eqType_X (type sig)),
